

# ECO2100 Part 2 Homework 1

Derek Caughy

November 13, 2025

a)

Social welfare is given by:

$$S = \overbrace{f(k)(1-u)}^{\text{Production of firm in match}} - \underbrace{vk}_{\text{total cost of vacancies}}$$

$\downarrow$  (from  $f(k)(1-u)$ )       $\downarrow$  (from  $m(\lambda)u$ )       $\uparrow$  (to  $vk$ )  
 Number of matches

Note that we want to solve the steady state level of unemployment. First note that

$$\underbrace{\dot{u}}_{\text{change in unemployment across time, =0 in steady state}} = \delta(1-u) - \underbrace{\frac{m(\lambda)}{\lambda}u}_{\text{mathcing rate of unemployed workers times unemployed}}$$

$\uparrow$  (to  $\delta(1-u)$ )       $\downarrow$  (from  $\frac{m(\lambda)}{\lambda}u$ )  
 rate of job destruction times employed

Thus in steady state:

$$0 = \delta - \left(\delta + \frac{m(\lambda)}{\lambda}\right)u$$

$$\iff u = \frac{\delta}{\delta + \frac{m(\lambda)}{\lambda}} = \frac{\lambda\delta}{\lambda\delta + m(\lambda)}$$

Furthermore, note that

$$\lambda = \frac{u}{v} \iff v = \frac{u}{\lambda} = \frac{\delta}{\lambda\delta + m(\lambda)}$$

Thus we can write the social planner's problem

$$\max_{\lambda \geq 0, k > 0} f(k) \frac{m(\lambda)}{\lambda\delta + m(\lambda)} - k \frac{\delta}{\lambda\delta + m(\lambda)}$$

The Lagrangian can be written as:

$$\mathcal{L}(\lambda, k, \mu_1, \mu_2) = \frac{f(k)m(\lambda) - k\delta}{\lambda\delta + m(\lambda)} + \mu_1(k - \epsilon) + \mu_2\lambda$$

where  $\epsilon > 0$  is an arbitrary constant.

**b)**

First note, that  $\epsilon$  is arbitrary, therefore we can always choose some  $\epsilon$  such that  $k > \epsilon > 0$ , thus by complementary slackness  $\mu_1 = 0$ . Secondly, for finite The first order conditions are written as follows:

$$\frac{f'(k)m(\lambda) - \delta}{\lambda\delta + m(\lambda)} = 0 \quad (k)$$

$$\frac{f(k)m'(\lambda)(\lambda\delta + m(\lambda)) - (\delta + m'(\lambda))(f(k)m(\lambda) - k\delta)}{(\lambda\delta + m(\lambda))^2} + \mu_2 = 0 \quad (\lambda)$$

Inspecting condition (k) and taking the limit as  $\lambda \rightarrow 0$  reveals that  $\lambda \neq 0$ . That is,

$$\lim_{\lambda \rightarrow 0} \frac{f'(k)m(\lambda) - \delta}{\lambda\delta + m(\lambda)} = \frac{-\delta}{\infty} < 0$$

By complementary slackness, it follows that  $\mu_2 = 0$  Now inspect FOC ( $\lambda$ ) we can derive:

$$f(k)m'(\lambda)(\lambda\delta + m(\lambda)) - (\delta + m'(\lambda))(f(k)m(\lambda) - k\delta) = 0$$

by the denominator necessairily being nonzero. This can be simplified:

$$\begin{aligned} \lambda f(k)m'(\lambda) - f(k)m(\lambda) + k(\delta + m'(\lambda)) &= 0 \\ \iff (\lambda m'(\lambda) - m(\lambda))f(k) + k(\delta + m'(\lambda)) &= 0 \\ \iff \left(1 - \frac{m(\lambda)}{\lambda m'(\lambda)}\right)f(k) + k\left(\frac{\delta}{\lambda m'(\lambda)} + \frac{1}{\lambda}\right) &= 0 \end{aligned}$$

Define

$$\eta(\lambda) = \frac{m(\lambda)}{\lambda m'(\lambda)}$$

Then re-write the above:

$$(1 - \eta(\lambda)) + k(\delta\eta(\lambda)m(\lambda) +)$$

**c)**

$$rJ(k) = f(k) - w - \delta(J(k) - V(k)) \quad (i)$$

$$rV(k) = -k + m(\lambda)(J(k) - V(k)) \quad (ii)$$

$$rW(k) = w - \delta(W(k) - U(k)) \quad (iii)$$

$$rU(k) = \frac{m(\lambda)}{\lambda}(W(k) - U(k)) \quad (iv)$$

**d)**

First, note that by  $k = \bar{k}$  that the above Bellman equations are no longer functions of  $k$ . Furthermore, the equilibrium wage rate will be given by Nash Bargaining. That is

$$\begin{aligned} w &= \arg \max_{\beta} (W - U)^{\beta} (J - V)^{(1-\beta)} \\ &= \arg \max_{\beta} \beta \ln(W - U) + (1 - \beta) \ln(J - V) \end{aligned}$$

The first order condition yields:

$$\beta \frac{\partial W}{\partial w} + (1 - \beta) \frac{\partial J}{\partial w} = 0$$

The partial derivatives come from the fact that  $W$  and  $J$  are functions of  $w$ , while  $V$  and  $U$  are not. Re-writing iii:

$$W = \frac{w - \delta U}{r + \delta}$$

Doing the same for  $J$  in terms of  $i$  yields:

$$J = \frac{f(k) - w - \delta V}{r + \delta}$$

It becomes obvious that  $\frac{\partial W}{\partial w} = -\frac{\partial J}{\partial w}$  thus the first order condition can be re-written:

$$\begin{aligned} \beta \frac{1}{W - U} - (1 - \beta) \frac{1}{J - V} &= 0 \\ \iff \beta(J - V) &= (1 - \beta)(W - U) \end{aligned}$$

Now we note the free entry condition which means that  $V = 0$  we can re-write the FOC to be:

$$\begin{aligned} W - U &= \beta(W - U + J) \\ &\quad \begin{array}{c} \uparrow \text{blue} \quad \quad \quad \uparrow \text{red} \\ = \frac{w - rU}{r + \delta} \text{ from iii} \quad \quad = \frac{f(k) - w}{r + \delta} \text{ from i} \end{array} \\ \iff \frac{w - rU}{r + \delta} &= \frac{\beta}{r + \delta} (f(k) - rU) \\ \iff rU(\beta - 1) &= \beta f(k) - w \end{aligned} \quad \text{(garbage)}$$

From the FOC we can also derive:

$$W - U = \frac{\beta}{1 - \beta} J$$

From ii we can obtain

$$J = \frac{k}{m(\lambda)}$$

Thus:

$$W - U = \frac{\beta}{1 - \beta} \frac{k}{m(\lambda)}$$

Which can be substituted into iv to obtain

$$rU = \frac{m(\lambda)}{\lambda} \frac{\beta}{1 - \beta} \frac{k}{m(\lambda)} = \frac{\beta}{1 - \beta} \frac{k}{\lambda}$$

Substituting into garbage and doing some simplifying:

$$\begin{aligned} -\beta \frac{k}{\lambda} &= \beta f(k) - w \\ \iff w &= \beta \left( f(k) + \frac{k}{\lambda} \right) \end{aligned}$$

Now inspect ii using  $J$  from i

$$\begin{aligned} 0 &= -k + m(\lambda) \frac{f(k) - w}{r + \delta} \\ \iff w &= f(k) - \frac{r + \delta}{m(\lambda)} k \end{aligned}$$

Thus

$$\begin{aligned} \beta \left( f(k) + \frac{k}{\lambda} \right) &= f(k) - \frac{r + \delta}{m(\lambda)} k \\ \iff (1 - \beta) f(k) - k \left( \frac{\beta}{\lambda} + \frac{r + \delta}{m(\lambda)} \right) &= 0 \end{aligned}$$